proof/invariants/isBuiltFromWriteAccessibleRec.v
@@ -6320,6 +6320,219 @@ revert buildPart parentsList s0. induction statesList; simpl; intros buildPart p
   rewrite <-beqAddrFalse in *. rewrite removeDupIdentity in *; auto.
 Qed.
 
+Lemma PDTisNoConfigInChildPreservedIsBuilt s s1 s0 pdAddr pdentry1 blockInParentPartitionAddr bentry newMPU flag:
+PDTisNoConfigInChild s0
+-> PDTIfPDFlag s0
+-> multiplexerIsPDT s0
+-> wellFormedFstShadowIfBlockEntry s0
+-> noDupPartitionTree s0
+-> lookup pdAddr (memory s0) beqAddr = Some (PDT pdentry1)
+-> lookup blockInParentPartitionAddr (memory s0) beqAddr = Some (BE bentry)
+-> (false = checkChild blockInParentPartitionAddr s0 (CPaddr (blockInParentPartitionAddr + sh1offset))
+    \/ flag = false)
+-> (s = s1
+    \/
+     s =
+     {|
+       currentPartition := currentPartition s1;
+       memory :=
+         add pdAddr
+           (PDT
+              {|
+                structure := structure pdentry1;
+                firstfreeslot := firstfreeslot pdentry1;
+                nbfreeslots := nbfreeslots pdentry1;
+                nbprepare := nbprepare pdentry1;
+                parent := ADT.parent pdentry1;
+                MPU := newMPU;
+                vidtAddr := vidtAddr pdentry1
+              |}) (memory s1) beqAddr
+     |})
+-> s1 =
+      {|
+        currentPartition := currentPartition s0;
+        memory :=
+          add blockInParentPartitionAddr
+            (BE
+               (CBlockEntry (read bentry) (write bentry) (exec bentry) (present bentry) flag
+                  (blockindex bentry) (blockrange bentry))) (memory s0) beqAddr
+      |}
+-> PDTisNoConfigInChild s.
+Proof.
+intros HPDTNoConfig HPDTIfPDFlag HmultIsPDT Hwell HnoDupTree HlookupPd HlookupBlockP HflagOr HpropsOr Hs1 pdparent
+  child pdentry block sh1entryaddr addr HparentIsPart HchildIsPart HlookupChild HblockMapped Hsh1 HPDflag
+  HaddrInBlock.
+assert(HgetPartsEq: getPartitions multiplexer s = getPartitions multiplexer s0).
+{ revert HpropsOr Hs1. apply getPartitionsEqIsBuilt; auto. }
+rewrite HgetPartsEq in *.
+destruct (beqAddr blockInParentPartitionAddr pdAddr) eqn:HbeqBlockPdAddr.
+{
+  rewrite <-DTL.beqAddrTrue in HbeqBlockPdAddr. rewrite HbeqBlockPdAddr in *. exfalso; congruence.
+}
+assert(HlookupPds1: lookup pdAddr (memory s1) beqAddr = Some (PDT pdentry1)).
+{
+  rewrite Hs1. simpl. rewrite HbeqBlockPdAddr. rewrite <-beqAddrFalse in HbeqBlockPdAddr.
+  rewrite removeDupIdentity; auto.
+}
+assert(HlookupChilds0: exists pdentry0, lookup child (memory s0) beqAddr = Some (PDT pdentry0)
+  /\ structure pdentry = structure pdentry0).
+{
+  assert(HlookupChilds1: exists pdentry0, lookup child (memory s1) beqAddr = Some (PDT pdentry0)
+    /\ structure pdentry = structure pdentry0).
+  {
+    destruct HpropsOr as [Heq | Hs].
+    - subst s. exists pdentry. auto.
+    - rewrite Hs in HlookupChild. simpl in *. destruct (beqAddr pdAddr child) eqn:HbeqParts.
+      + exists pdentry1. rewrite <-DTL.beqAddrTrue in HbeqParts. subst child. injection HlookupChild as HpdentriesEq.
+        subst pdentry. auto.
+      + exists pdentry. rewrite <-beqAddrFalse in *. rewrite removeDupIdentity in *; auto.
+  }
+  destruct HlookupChilds1 as [pdentry0 (HlookupChilds1 & HstructEq)]. exists pdentry0. rewrite Hs1 in HlookupChilds1.
+  simpl in *. destruct (beqAddr blockInParentPartitionAddr child) eqn:HbeqBlockChild; try(exfalso; congruence).
+  rewrite <-beqAddrFalse in *. rewrite removeDupIdentity in *; auto.
+}
+destruct HlookupChilds0 as [pdentry0 (HlookupChilds0 & HstructEq)]. rewrite HstructEq.
+assert(HgetMappedEq: forall partition, isPDT partition s0
+  -> getMappedBlocks partition s = getMappedBlocks partition s0).
+{ intros partition HpartBIsPDT. revert HpropsOr Hs1. apply getMappedBlocksEqIsBuilt; auto. }
+assert(isPDT pdparent s0) by (apply partitionsArePDT; trivial).
+rewrite HgetMappedEq in *; trivial. assert(HgetChildrenEq: getChildren pdparent s = getChildren pdparent s0).
+{ revert HpropsOr Hs1. apply getChildrenEqIsBuilt; trivial. }
+rewrite HgetChildrenEq in *.
+assert(Hblocks0: sh1entryAddr block sh1entryaddr s0 /\ In addr (getAllPaddrAux [block] s0)).
+{
+  assert(Hblocks1: sh1entryAddr block sh1entryaddr s1 /\ In addr (getAllPaddrAux [block] s1)).
+  {
+    destruct HpropsOr as [Heq | Hs]; try(subst s; split; assumption). unfold sh1entryAddr in *. rewrite Hs in Hsh1.
+    rewrite Hs in HaddrInBlock. simpl in *. destruct (beqAddr pdAddr block) eqn:HbeqPdBlock; try(exfalso; congruence).
+    rewrite <-beqAddrFalse in *. rewrite removeDupIdentity in *; auto.
+  }
+  destruct Hblocks1 as (Hsh1s1 & HaddrInBlocks1). rewrite Hs1 in HaddrInBlocks1.
+  unfold sh1entryAddr in *. rewrite Hs1 in Hsh1s1. simpl in *.
+  destruct (beqAddr blockInParentPartitionAddr block) eqn:HbeqBlocks.
+  - rewrite <-DTL.beqAddrTrue in HbeqBlocks. subst block. rewrite HlookupBlockP.
+    assert(blockindex bentry < kernelStructureEntriesNb) by (apply Hidx). unfold CBlockEntry in HaddrInBlocks1.
+    destruct (Compare_dec.lt_dec (blockindex bentry) kernelStructureEntriesNb); try(lia). auto.
+  - rewrite <-beqAddrFalse in *. rewrite removeDupIdentity in *; auto.
+}
+destruct Hblocks0 as (Hsh1s0 & HaddrInBlocks0).
+assert(HPDflags0: sh1entryPDflag sh1entryaddr true s0).
+{
+  unfold sh1entryPDflag in *.
+  assert(Heq: lookup sh1entryaddr (memory s) beqAddr = lookup sh1entryaddr (memory s1) beqAddr).
+  {
+    destruct HpropsOr as [Heq | Hs]; try(subst s; reflexivity). rewrite Hs. rewrite Hs in HPDflag. simpl in *.
+    destruct (beqAddr pdAddr sh1entryaddr) eqn:HbeqPartSh1; try(exfalso; congruence).
+    rewrite <-beqAddrFalse in *. rewrite removeDupIdentity; auto.
+  }
+  rewrite Heq in *. rewrite Hs1 in HPDflag. simpl in *.
+  destruct (beqAddr blockInParentPartitionAddr sh1entryaddr) eqn:HbeqBlockSh1; try(exfalso; congruence).
+  rewrite <-beqAddrFalse in *. rewrite removeDupIdentity in *; auto.
+}
+specialize(HPDTNoConfig pdparent child pdentry0 block sh1entryaddr addr HparentIsPart HchildIsPart HlookupChilds0
+  HblockMapped Hsh1s0 HPDflags0 HaddrInBlocks0).
+assert(HeqConfig: getConfigBlocksAux (maxIdx + 1) (structure pdentry0) s (CIndex maxNbPrepare)
+  = getConfigBlocksAux (maxIdx + 1) (structure pdentry0) s0 (CIndex maxNbPrepare)).
+{
+  assert(Heq: getConfigBlocksAux (maxIdx + 1) (structure pdentry0) s (CIndex maxNbPrepare)
+    = getConfigBlocksAux (maxIdx + 1) (structure pdentry0) s1 (CIndex maxNbPrepare)).
+  {
+    destruct HpropsOr as [Heq | Hs]; try(subst s; reflexivity). rewrite Hs.
+    apply getConfigBlocksAuxEqPDT. unfold isPDT. rewrite HlookupPds1. trivial.
+  }
+  rewrite Heq. rewrite Hs1. apply getConfigBlocksAuxEqBE. unfold isBE. rewrite HlookupBlockP. trivial.
+}
+rewrite HeqConfig. assert(HeqPaddrs1: getAllPaddrConfigAux (filterOptionPaddr
+  (getConfigBlocksAux (maxIdx + 1) (structure pdentry0) s0 (CIndex maxNbPrepare))) s
+  = getAllPaddrConfigAux (filterOptionPaddr
+    (getConfigBlocksAux (maxIdx + 1) (structure pdentry0) s0 (CIndex maxNbPrepare))) s1).
+{
+  destruct HpropsOr as [Heq | Hs]; try(subst s; reflexivity). rewrite Hs.
+  apply getAllPaddrConfigAuxEqPDT. unfold isPDT. rewrite HlookupPds1. trivial.
+}
+rewrite HeqPaddrs1. rewrite Hs1. rewrite getAllPaddrConfigAuxEqBE; trivial. unfold isBE. rewrite HlookupBlockP.
+trivial.
+Qed.
+
+Lemma PDTisNoConfigInChildPreservedIsBuiltRec s s0 statesList parentsList buildPart startaddr endaddr flag:
+multiplexerIsPDT s0
+-> wellFormedFstShadowIfBlockEntry s0
+-> noDupPartitionTree s0
+-> PDTIfPDFlag s0
+-> PDTisNoConfigInChild s0
+-> (~isPDT startaddr s0 \/ flag = false)
+-> isBuiltFromWriteAccessibleRec s0 s statesList parentsList buildPart startaddr endaddr flag
+-> PDTisNoConfigInChild s.
+Proof.
+revert buildPart parentsList s0. induction statesList; simpl; intros buildPart parentsList s0
+  HmultIsPDT HwellSh1 HnoDupTree HPDTIfPDFlag HPDTNotInConfig HflagProps HisBuilt.
+- destruct HisBuilt as [_ Hss0Eq]. subst s. intuition.
+- destruct HisBuilt as [pdAddr (newPdEntriesList & (HparentsList & (realMPU & (pdentry0 & pdentry1 &
+                      (blockInParentPartitionAddr & (bentry & (newBentry & (s1 & (Hs1 & (HpropsOr
+                       & (HnewB & (HlookupBlocks0 & HlookupBlocks1 & HPFlag & HblockStart & HblockEnd &
+                       HpdIsPart & HblockIsMapped & HlookupParentsInit & HlookupParents1 & HlookupAncestorsInit &
+                       HlookupAncestors1 & Hancestor & HbaseNotRoot & HisBuilt))))))))))))].
+  assert(HflagPropsB: false = checkChild blockInParentPartitionAddr s0 (CPaddr (blockInParentPartitionAddr+sh1offset))
+    \/ flag = false).
+  {
+    destruct HflagProps as [HstartNotPDT | HflagFalse]; auto. left.
+    destruct (checkChild blockInParentPartitionAddr s0 (CPaddr (blockInParentPartitionAddr+sh1offset)))
+      eqn:HcheckChild; trivial. exfalso.
+    assert(Hchild: true = checkChild blockInParentPartitionAddr s0 (CPaddr (blockInParentPartitionAddr+sh1offset))
+      /\ sh1entryAddr blockInParentPartitionAddr (CPaddr (blockInParentPartitionAddr+sh1offset)) s0).
+    { split; auto. unfold sh1entryAddr. rewrite HlookupBlocks0. reflexivity. }
+    specialize(HPDTIfPDFlag blockInParentPartitionAddr (CPaddr (blockInParentPartitionAddr+sh1offset)) pdAddr
+      HpdIsPart HblockIsMapped Hchild). destruct HPDTIfPDFlag as (_ & _ & [startBis (HstartBis & HstartBIsPDT)]).
+    unfold bentryStartAddr in *. unfold entryPDT in *. rewrite HlookupBlocks0 in *. rewrite <-HblockStart in *.
+    subst startBis. contradict HstartNotPDT. unfold isPDT.
+    destruct (lookup startaddr (memory s0) beqAddr); try(congruence).
+    destruct v; try(congruence). trivial.
+  }
+  assert(HpropsA: PDTisNoConfigInChild a).
+  {
+    apply PDTisNoConfigInChildPreservedIsBuilt with s1 s0 pdAddr pdentry1 blockInParentPartitionAddr bentry
+        (MAL.removeBlockFromPhysicalMPUAux blockInParentPartitionAddr realMPU) flag; trivial; intuition.
+  }
+  assert(multiplexerIsPDT a).
+  {
+    revert Hs1. apply multiplexerIsPDTPreservedIsBuilt with pdAddr pdentry1
+      (MAL.removeBlockFromPhysicalMPUAux blockInParentPartitionAddr realMPU); trivial.
+    destruct HpropsOr as [Heq | (Ha & _)]; auto.
+  }
+  assert(wellFormedFstShadowIfBlockEntry a).
+  {
+    revert Hs1. apply wellFormedFstShadowIfBlockEntryPreservedIsBuilt with pdAddr pdentry1
+      (MAL.removeBlockFromPhysicalMPUAux blockInParentPartitionAddr realMPU); trivial.
+    destruct HpropsOr as [Heq | (Ha & _)]; auto.
+  }
+  assert(HgetPartsEq: getPartitions multiplexer a = getPartitions multiplexer s0).
+  {
+    revert Hs1. apply getPartitionsEqIsBuilt with pdAddr pdentry1
+      (MAL.removeBlockFromPhysicalMPUAux blockInParentPartitionAddr realMPU); trivial.
+    destruct HpropsOr as [Heq | (Ha & _)]; auto.
+  }
+  assert(noDupPartitionTree a).
+  { unfold noDupPartitionTree. rewrite HgetPartsEq. assumption. }
+  assert(PDTIfPDFlag a).
+  {
+    revert Hs1. apply PDTIfPDFlagPreservedIsBuilt with pdAddr pdentry1
+      (MAL.removeBlockFromPhysicalMPUAux blockInParentPartitionAddr realMPU); trivial.
+    destruct HpropsOr as [Heq | (Ha & _)]; auto.
+  }
+  apply IHstatesList with pdAddr newPdEntriesList a; trivial.
+  destruct HflagProps as [HstartNotPDT | HflagFalse]; auto. left. contradict HstartNotPDT.
+  assert(HstartNotPDTs1: isPDT startaddr s1).
+  {
+    destruct HpropsOr as [Heq | (Ha & _)]; try(subst a; assumption). unfold isPDT in *. rewrite Ha in HstartNotPDT.
+    simpl in *. destruct (beqAddr pdAddr startaddr) eqn:HbeqPdStart.
+    - rewrite <-DTL.beqAddrTrue in HbeqPdStart. subst startaddr. rewrite HlookupAncestors1. trivial.
+    - rewrite <-beqAddrFalse in *. rewrite removeDupIdentity in *; auto.
+  }
+  unfold isPDT in *. rewrite Hs1 in HstartNotPDTs1. simpl in *.
+  destruct (beqAddr blockInParentPartitionAddr startaddr) eqn:HbeqBlockStart; try(exfalso; congruence).
+  rewrite <-beqAddrFalse in *. rewrite removeDupIdentity in *; auto.
+Qed.
+
 (** General properties on important tools **)
 
 Lemma lookupBENotPresEqWriteAccess addr startaddr endaddr statesList initState parentsList pdparent flag s:
